end of day 29/04/19

inference-tool/src/main/scala/inference/Dirties.scala
@@ -137,18 +137,39 @@ object Dirties {
     case Value.Numa(n) => s"NUM(${valueOf(n)})"
   }
 
-  def generaliseOutputContextCheck(e: iEFSM, r: Nat.nat, v: Value.value, s: Nat.nat): Boolean = {
-    val f = "intermediate_"+System.currentTimeMillis()
-    TypeConversion.efsmToSALTranslator(Inference.tm(e), f)
 
-    addLTL("salfiles/" + f + ".sal", s"  generaliseOutput: THEOREM MichaelsEFSM |- G(cfstate = State_${valueOf(s)} => r_${valueOf(r)} = Some(${salValue(v)}));")
+  // TODO: Convert the old EFSM to SAL and check
+  //         U(cfstate /= NULL_STATE, cfstate=State_2) =>
+  //         U(label = coin => I(1) = NUM(50), X(cfstate = NULL_STATE));
+  //       Then convert the new EFSM and check
+  //         U(cfstate /= NULL_STATE, cfstate = State_1) =>
+  //         U(label = select => I(1) = STR(String_coke), cfstate = NULL_STATE) =>
+  //         U(cfstate = State_1 => r_1 = Some(STR(String_coke)), cfstate=NULL_STATE);
+  def generaliseOutputContextCheck(l: String, ePrime: iEFSM, e: iEFSM, r: Nat.nat, v: Value.value, s_old: Nat.nat, s_new: Nat.nat): Boolean = {
+    val f_old = "orig_"+System.currentTimeMillis()
+    TypeConversion.efsmToSALTranslator(Inference.tm(e), f_old)
+    val inxLabel = Code_Generation.input_updates_register(ePrime)
+    addLTL("salfiles/" + f_old + s".sal", s"  inputValue: THEOREM MichaelsEFSM |-\n" +
+      s"U(cfstate /= NULL_STATE, cfstate=State_${valueOf(s_old)}) =>\n"+
+      s"U(label = ${inxLabel._2} => I(1) = ${salValue(v)}, X(cfstate = NULL_STATE));")
 
-    val output = Seq("bash", "-c", "cd salfiles; sal-smc --assertion='" + f + "{100}!generaliseOutput'").!!
-    println("sal-smc --assertion='" + f + "{100}!generaliseOutput'")
-    if (output.toString != "proved.\n") {
-      print(output)
-    }
-    return (output.toString == "proved.\n")
+    val f_new = "intermediate_"+System.currentTimeMillis()
+    TypeConversion.efsmToSALTranslator(Inference.tm(ePrime), f_new)
+    addLTL("salfiles/" + f_new + ".sal", s"  generaliseOutput: THEOREM MichaelsEFSM |-\n"+
+      s"U(cfstate /= NULL_STATE, cfstate = State_${valueOf(s_new)}) =>\n"+
+      s"U(label = select => I(${valueOf(inxLabel._1)}) = ${salValue(v)}, cfstate = NULL_STATE) =>\n"+
+      s"U(cfstate = State_${valueOf(s_new)} => r_1 = Some(${salValue(v)}), cfstate=NULL_STATE);")
+
+
+    println(s"sal-smc --assertion='${f_old}{100}!inputValue'")
+    val output1 = Seq("bash", "-c", s"cd salfiles; sal-smc --assertion='${f_old}{100}!inputValue'").!!
+    println(output1)
+
+    println(s"sal-smc --assertion='${f_new}{100}!generaliseOutput'")
+    val output2 = Seq("bash", "-c", s"cd salfiles; sal-smc --assertion='${f_new}{100}!generaliseOutput'").!!
+    println(output2)
+
+    return (output1.toString == "proved.\n" && output2.toString == "proved.\n")
   }
 
   def scalaDirectlySubsumes(a: iEFSM,
@@ -175,12 +196,12 @@ object Dirties {
                                 println("n")
                                 return false
                               }
-                              else if (Store_Reuse_Subsumption.generalise_output_direct_subsumption(t1, t2, b, s_prime)) {
+                              else if (Store_Reuse_Subsumption.generalise_output_direct_subsumption(t1, t2, b, a, s, s_prime)) {
                                 // This needs modifying to model check but it should be OK for now
                                 println("y")
                                 return true
                               }
-                              else if (Store_Reuse_Subsumption.generalise_output_direct_subsumption(t2, t1, b, s_prime)) {
+                              else if (Store_Reuse_Subsumption.generalise_output_direct_subsumption(t2, t1, b, a, s, s_prime)) {
                                 // This needs modifying to model check but it should be OK for now
                                 println("n")
                                 return false
